more commit

TestSamples/Lecture3.v
@@ -2,7 +2,14 @@ Require Import Arith Lia List String.
 Import ListNotations.
 Open Scope string.
 
+Definition eq_dec (A : Type) :=
+  forall (x : A),
+    forall (y : A),
+      {x = y} + {x <> y}.
+
+
 Notation var := string.
+Definition var_eq : eq_dec var := string_dec.
 
 Inductive arith : Set :=
 | Const (n : nat)
@@ -26,3 +33,219 @@ Proof.
     (*Another flavor of destruct called inversion*)
     inversion Heq.
 Qed.
+
+Fixpoint has_zero (e : arith) : bool :=
+  match e with
+  | Const n => Nat.eqb n 0
+  | Var x => false
+  | Plus e1 e2  => has_zero e1 || has_zero e2
+  | Minus e1 e2 => has_zero e1 || has_zero e2
+  | Times e1 e2 => has_zero e1 || has_zero e2
+  end.
+
+Compute has_zero (Const 0). (* true *)
+Compute has_zero (Const 1). (* false *)
+Compute has_zero (Plus (Var "x") (Var "y")). (* false *)
+Compute has_zero (Minus (Plus (Var "x") (Var "y")) (Const 0)). (* true *)
+
+Declare Scope arith_scope. (* defines a name for our collection of notations *)
+Coercion Const : nat >-> arith.
+Coercion Var : var >-> arith.
+Infix "+" := Plus : arith_scope.
+Infix "-" := Minus : arith_scope.
+Infix "*" := Times : arith_scope.
+Delimit Scope arith_scope with arith. (* lets us use "%arith" annotations *)
+Bind Scope arith_scope with arith.
+
+(* Now let's see those same examples again. *)
+Compute has_zero 0. (* true *)
+Compute has_zero 1. (* false *)
+Compute has_zero ("x" + "y")%arith. (* false *)
+Compute has_zero ("x" + "y" - 0)%arith. (* true *)
+
+(* memory *)
+Definition valuation := list (var * nat).
+
+Fixpoint lookup (x : var) (v : valuation) : option nat :=
+  match v with
+  | [] => None
+  | (y, n) :: v' =>
+    if var_eq x y
+    then Some n
+    else lookup x v'
+  end.
+
+Fixpoint eval_arith (e : arith) (v : valuation) : nat :=
+  match e with
+  | Const n => n
+  | Var x =>
+    match lookup x v with
+    | None => 0  (* sorta bogus! *)
+    | Some n => n
+    end
+  | Plus  e1 e2 => eval_arith e1 v + eval_arith e2 v
+  | Minus e1 e2 => eval_arith e1 v - eval_arith e2 v
+  | Times e1 e2 => eval_arith e1 v * eval_arith e2 v
+  end.
+
+Compute eval_arith (1 + 1)%arith [].  (* 2 *)
+Compute eval_arith (2)%arith [].      (* also 2 *)
+
+Locate "+".
+
+Lemma eval_one_plus_one_is_eval_two :
+  forall v,
+    eval_arith (1 + 1)%arith v = eval_arith 2 v.
+Proof.
+  intro.
+  simpl.
+  reflexivity.
+Qed.
+
+
+(* from expressions to commands *)
+Inductive cmd :=
+| Skip
+| Assign (x : var) (e : arith)
+| Sequence (c1 c2 : cmd)
+| Repeat (e : arith) (body : cmd).
+
+Fixpoint do_n_times {A} (f : A -> A) (n : nat) (x : A) : A :=
+  match n with
+  | O => x
+  | S n' => do_n_times f n' (f x)
+  end.
+
+Compute do_n_times (cons true) 7 [false; false]. (* 7 "true"s followed by 2 "false"s *)
+
+Fixpoint eval_cmd (c : cmd) (v : valuation) : valuation :=
+  match c with
+  | Skip => v
+  | Assign x e => (x, eval_arith e v) :: v
+  | Sequence c1 c2 => eval_cmd c2 (eval_cmd c1 v) 
+  | Repeat e body => do_n_times (eval_cmd body) (eval_arith e v) v
+  (* | Repeat e body => do_n_times (fun v => eval_cmd body v) (eval_arith e v) v *)
+  end.
+
+(* more notation *)
+Declare Scope cmd_scope.
+Delimit Scope cmd_scope with cmd.
+Bind Scope cmd_scope with cmd.
+Notation "x <- e" := (Assign x e%arith) (at level 75) : cmd_scope.
+Infix ";" := Sequence (at level 76) : cmd_scope.
+Notation "'repeat' e 'doing' body 'done'" :=
+  (Repeat e%arith body) (at level 75) : cmd_scope.
+
+Fixpoint factorial_tr (n : nat) (acc : nat) : nat :=
+  match n with
+  | O => acc
+  | S m => factorial_tr m (n * acc)
+  end.
+
+Definition factorial_tailrec (n : nat) : nat :=
+  factorial_tr n 1.
+
+
+
+
+
+
+Definition factorial : cmd :=
+  "output" <- 1;
+  repeat "input" doing
+    "output" <- "output" * "input";
+    "input" <- "input" - 1
+  done.
+
+
+Print factorial.
+(* if we put 4 in "input", then will compute 4 * 3 * 2 * 1 in "output" *)
+
+Fixpoint coq_factorial (n : nat) : nat :=
+  match n with
+  | 0 => 1
+  | S n' => n * coq_factorial n'
+  end.
+
+Compute coq_factorial 4.
+
+Theorem factorial_correct :
+  forall v n,
+    lookup "input" v = Some n ->
+    lookup "output" (eval_cmd factorial v) = Some (coq_factorial n).
+Proof.
+  intros.
+  unfold factorial.
+  simpl.
+Qed.
+
+
+
+
+
+
+
+Definition factorial_loop_body : cmd :=
+  "output" <- "output" * "input";
+  "input" <- "input" - 1.
+
+Theorem factorial_ok :
+  forall v input,
+    lookup "input" v = Some input ->
+    lookup "output" (eval_cmd factorial v) = Some (factorial_tailrec input).
+Proof.
+  (* motto... *)
+  intros v input Hinput.
+  unfold factorial, factorial_tailrec.
+  fold factorial_loop_body.
+  cbn -[factorial_loop_body].
+  (* do_n_times (eval_cmd factorial_loop_body) *)
+Abort.
+
+Definition map_equiv m1 m2 := forall x, lookup x m1 = lookup x m2.
+
+Example map_equiv_example :
+  forall m,
+    map_equiv (("x", 0) :: ("y", 1) :: m) (("y", 1) :: ("x", 0) :: m).
+Proof.
+  (* example of destructing on a non-variable *)
+Admitted.
+
+Ltac solve_map_cases :=
+  unfold map_equiv; intros; simpl;
+  repeat destruct (var_eq _ _); try congruence.
+
+(* key lemma for factorial *)
+Lemma factorial_loop_body_ok :
+  forall n acc v,
+    lookup "input" v = Some n ->
+    lookup "output" v = Some acc ->
+    map_equiv
+      (do_n_times (eval_cmd factorial_loop_body) n v)
+      (("input", 0) :: ("output", factorial_tr n acc) :: v).
+Proof.
+  (* do_n_times is recursive on n. So is factorial_tr. Let's induct on n. *)
+  induction n; intros acc v Hinput Houtput x.
+  - simpl. solve_map_cases.
+  - cbn [do_n_times factorial_tr].
+    unfold map_equiv in *.
+    rewrite IHn with (acc := S n * acc); solve_map_cases.
+    + rewrite Hinput. f_equal. lia.
+    + rewrite Hinput, Houtput. f_equal. lia.
+Qed.
+
+Theorem factorial_ok :
+  forall v input,
+    lookup "input" v = Some input ->
+    lookup "output" (eval_cmd factorial v) = Some (factorial_tailrec input).
+Proof.
+  intros v input Hinput.
+  unfold factorial, factorial_tailrec.
+  fold factorial_loop_body.
+  cbn -[factorial_loop_body].
+  rewrite Hinput.
+  rewrite factorial_loop_body_ok with (acc := 1); solve_map_cases.
+Qed.
+
+
+
